name changes

theories/maps/grad_into_dyn/definition.v
@@ -1,10 +1,10 @@
 From main Require Import imports.
-From main.grad_lang Require Import types definition.
+From main.cast_calc Require Import types definition.
 From main.dyn_lang Require Import definition casts lib.
 
 (* The translation to define the semantics of surface language. *)
 
-Definition sf_expr := grad_lang.definition.expr .
+Definition sf_expr := cast_calc.definition.expr .
 
 Section expr.
 
@@ -12,21 +12,21 @@ Section expr.
 
   Fixpoint trns (e : sf_expr) : expr :=
     match e with
-    | grad_lang.definition.Lit b => Lit b
-    | grad_lang.definition.Seq e1 e2 => Seq ν (trns e1) (trns e2)
-    | grad_lang.definition.If e0 e1 e2 => If ν (trns e0) (trns e1) (trns e2)
-    | grad_lang.definition.BinOp binop e1 e2 => BinOp ν binop (trns e1) (trns e2)
-    | grad_lang.definition.Var v => Var v
-    | grad_lang.definition.Lam e => Lam (trns e)
-    | grad_lang.definition.App e1 e2 => App ν (trns e1) (trns e2)
-    | grad_lang.definition.InjL e => InjL (trns e)
-    | grad_lang.definition.InjR e => InjR (trns e)
-    | grad_lang.definition.Case e0 e1 e2 => Case ν (trns e0) (trns e1) (trns e2)
-    | grad_lang.definition.Fst e => Fst ν (trns e)
-    | grad_lang.definition.Snd e => Snd ν (trns e)
-    | grad_lang.definition.Pair e1 e2 => Pair (trns e1) (trns e2)
+    | cast_calc.definition.Lit b => Lit b
+    | cast_calc.definition.Seq e1 e2 => Seq ν (trns e1) (trns e2)
+    | cast_calc.definition.If e0 e1 e2 => If ν (trns e0) (trns e1) (trns e2)
+    | cast_calc.definition.BinOp binop e1 e2 => BinOp ν binop (trns e1) (trns e2)
+    | cast_calc.definition.Var v => Var v
+    | cast_calc.definition.Lam e => Lam (trns e)
+    | cast_calc.definition.App e1 e2 => App ν (trns e1) (trns e2)
+    | cast_calc.definition.InjL e => InjL (trns e)
+    | cast_calc.definition.InjR e => InjR (trns e)
+    | cast_calc.definition.Case e0 e1 e2 => Case ν (trns e0) (trns e1) (trns e2)
+    | cast_calc.definition.Fst e => Fst ν (trns e)
+    | cast_calc.definition.Snd e => Snd ν (trns e)
+    | cast_calc.definition.Pair e1 e2 => Pair (trns e1) (trns e2)
     | Cast ℓ τ1 τ2 e => App ν (of_val $ cast' ℓ τ1 τ2) (trns e)
-    | grad_lang.definition.Error ℓ => Error ℓ
+    | cast_calc.definition.Error ℓ => Error ℓ
     end.
 
 End expr.
@@ -35,34 +35,34 @@ Notation "⟨ e ⟩" := (trns e).
 (* corresponds to ⌊ _ ⌋ in paper; latter is quite confusing in unicode though so we avoid it *)
 
 
-From main.grad_lang Require Import contexts.
+From main.cast_calc Require Import contexts.
 From main.dyn_lang Require Import contexts.
 
 Section contexts.
 
   Context {ν : label} {Hν : NeverOccurs ν}.
 
-  Definition trns_ctx_item (Ci : grad_lang.contexts.ctx_item) : ctx_item :=
+  Definition trns_ctx_item (Ci : cast_calc.contexts.ctx_item) : ctx_item :=
     match Ci with
-    | grad_lang.contexts.CTX_Lam => CTX_Lam
-    | grad_lang.contexts.CTX_AppL e2 => CTX_AppL ν (trns e2)
-    | grad_lang.contexts.CTX_AppR e1 => CTX_AppR ν (trns e1)
-    | grad_lang.contexts.CTX_PairL e2 => CTX_PairL (trns e2)
-    | grad_lang.contexts.CTX_PairR e1 => CTX_PairR (trns e1)
-    | grad_lang.contexts.CTX_Fst => CTX_Fst ν
-    | grad_lang.contexts.CTX_Snd => CTX_Snd ν
-    | grad_lang.contexts.CTX_InjL => CTX_InjL
-    | grad_lang.contexts.CTX_InjR => CTX_InjR
-    | grad_lang.contexts.CTX_CaseL e1 e2 => CTX_CaseL ν (trns e1) (trns e2)
-    | grad_lang.contexts.CTX_CaseM e0 e2 => CTX_CaseM ν (trns e0) (trns e2)
-    | grad_lang.contexts.CTX_CaseR e0 e1 => CTX_CaseR ν (trns e0) (trns e1)
-    | grad_lang.contexts.CTX_BinOpL op e2 => CTX_BinOpL ν op (trns e2)
-    | grad_lang.contexts.CTX_BinOpR op e1 => CTX_BinOpR ν op (trns e1)
-    | grad_lang.contexts.CTX_IfL e1 e2 => CTX_IfL ν (trns e1) (trns e2)
-    | grad_lang.contexts.CTX_IfM e0 e2 => CTX_IfM ν (trns e0) (trns e2)
-    | grad_lang.contexts.CTX_IfR e0 e1 => CTX_IfR ν (trns e0) (trns e1)
-    | grad_lang.contexts.CTX_SeqL e2 => CTX_SeqL ν (trns e2)
-    | grad_lang.contexts.CTX_SeqR e1 => CTX_SeqR ν (trns e1)
+    | cast_calc.contexts.CTX_Lam => CTX_Lam
+    | cast_calc.contexts.CTX_AppL e2 => CTX_AppL ν (trns e2)
+    | cast_calc.contexts.CTX_AppR e1 => CTX_AppR ν (trns e1)
+    | cast_calc.contexts.CTX_PairL e2 => CTX_PairL (trns e2)
+    | cast_calc.contexts.CTX_PairR e1 => CTX_PairR (trns e1)
+    | cast_calc.contexts.CTX_Fst => CTX_Fst ν
+    | cast_calc.contexts.CTX_Snd => CTX_Snd ν
+    | cast_calc.contexts.CTX_InjL => CTX_InjL
+    | cast_calc.contexts.CTX_InjR => CTX_InjR
+    | cast_calc.contexts.CTX_CaseL e1 e2 => CTX_CaseL ν (trns e1) (trns e2)
+    | cast_calc.contexts.CTX_CaseM e0 e2 => CTX_CaseM ν (trns e0) (trns e2)
+    | cast_calc.contexts.CTX_CaseR e0 e1 => CTX_CaseR ν (trns e0) (trns e1)
+    | cast_calc.contexts.CTX_BinOpL op e2 => CTX_BinOpL ν op (trns e2)
+    | cast_calc.contexts.CTX_BinOpR op e1 => CTX_BinOpR ν op (trns e1)
+    | cast_calc.contexts.CTX_IfL e1 e2 => CTX_IfL ν (trns e1) (trns e2)
+    | cast_calc.contexts.CTX_IfM e0 e2 => CTX_IfM ν (trns e0) (trns e2)
+    | cast_calc.contexts.CTX_IfR e0 e1 => CTX_IfR ν (trns e0) (trns e1)
+    | cast_calc.contexts.CTX_SeqL e2 => CTX_SeqL ν (trns e2)
+    | cast_calc.contexts.CTX_SeqR e1 => CTX_SeqR ν (trns e1)
     | CTX_Cast ℓ τ1 τ2 => CTX_AppR ν (of_val $ cast' ℓ τ1 τ2)
         (* (CTX_AppR ν $ match consistency_decision τ1 τ2 with *)
         (*               | inl Pc => (of_val $ cast ℓ τ1 τ2 Pc) *)
@@ -70,14 +70,14 @@ Section contexts.
         (*               end) *)
     end.
 
-  Definition trns_ctx (C : grad_lang.contexts.ctx) : ctx :=
+  Definition trns_ctx (C : cast_calc.contexts.ctx) : ctx :=
     trns_ctx_item <$> C.
 
   Lemma trns_fill_ctx_item Ci e :
-    ⟨ grad_lang.contexts.fill_ctx_item Ci e ⟩ = fill_ctx_item (trns_ctx_item Ci) ⟨ e ⟩.
+    ⟨ cast_calc.contexts.fill_ctx_item Ci e ⟩ = fill_ctx_item (trns_ctx_item Ci) ⟨ e ⟩.
   Proof. destruct Ci; eauto. Qed.
   Lemma trns_fill_ctx C e :
-    ⟨ grad_lang.contexts.fill_ctx C e ⟩ = fill_ctx (trns_ctx C) ⟨ e ⟩.
+    ⟨ cast_calc.contexts.fill_ctx C e ⟩ = fill_ctx (trns_ctx C) ⟨ e ⟩.
   Proof. induction C; auto. by rewrite /= -IHC trns_fill_ctx_item. Qed.
 
   Lemma trns_ctx_app C C' : trns_ctx (C ++ C') = trns_ctx C ++ trns_ctx C'.
