theories/logrel/lemmas/compats.v
@@ -1,5 +1,5 @@
 From main.prelude Require Import imports autosubst big_op_three.
-From main.grad_lang Require Import types typing.
+From main.cast_calc Require Import types typing.
 From main.dyn_lang Require Import definition lemmas tactics lib casts contexts.
 From main.logrel Require Import definition.
 From main.logrel.lib Require Import weakestpre rfn small_helpers.
