theories/maps/dyn_embedding/typing.v
@@ -1,5 +1,5 @@
 From main.prelude Require Import imports autosubst big_op_three.
-From main.grad_lang Require Import types.
+From main.cast_calc Require Import types.
 From main.dyn_lang Require Import definition lemmas tactics labels lib.
 From main.logrel.lib Require Import weakestpre rfn small_helpers.
 
@@ -9,7 +9,7 @@ From iris.proofmode Require Import tactics.
 From main.logrel Require Import definition.
 From main.maps Require Import dyn_embedding.definition grad_into_dyn.definition.
 
-From main.grad_lang Require Import typing.
+From main.cast_calc Require Import typing.
 
 Section typing.
 
