theories/maps/linker/components/common.v
@@ -1,5 +1,5 @@
 From main.prelude Require Import imports base_lang.
-From main.grad_lang Require Import types.
+From main.cast_calc Require Import types.
 
 Definition LamN_type (Γ : list type) τ : type :=
   foldl (fun T t => Bin Arrow t T) τ Γ.
