theories/maps/linker/components/lemmas.v
@@ -1,4 +1,4 @@
-From main.grad_lang Require Import types labels.
+From main.cast_calc Require Import types labels.
 From main.dyn_lang Require Import definition casts lib tactics lemmas.
 From main.logrel Require Import rfn definition lib.small_helpers lemmas.casts_superfluous lemmas.fun_grad_into_dyn.
 From main.maps.linker.components Require Import common grd dyn agree.
